proof/SemProps.v
@@ -1,0 +1,243 @@
+Require Import CoqlibC.
+Require Import Simulation.
+Require Import LinkingC.
+Require Import Skeleton.
+Require Import Values.
+Require Import JMeq.
+Require Import Asmregs.
+Require Import Smallstep.
+Require Import Integers.
+
+Require Import Skeleton ModSem Mod Sem.
+Require Import SimSymb SimMem.
+
+Set Implicit Arguments.
+
+
+
+
+Section INITDTM.
+
+  Print fsim_properties.
+  Print determinate.
+
+  Context `{SM: SimMem.class}.
+  Context {SS: SimSymb.class SM}.
+  Variable p: program.
+  Let sem := Sem.semantics p.
+
+  Lemma system_disjoint
+        skenv_link
+        (WFBIG: SkEnv.wf skenv_link)
+        sys_def
+        fptr
+        (SYSTEM: Genv.find_funct (System.skenv skenv_link) fptr = Some (Internal sys_def))
+        md md_def
+        (MOD: In md p)
+        (MODSEM: Genv.find_funct (ModSem.skenv (Mod.get_modsem md skenv_link (Mod.data md))) fptr =
+                 Some (Internal md_def))
+    :
+      False
+  .
+  Proof.
+    erewrite <- Mod.get_modsem_projected_sk in *.
+    hexploit (SkEnv.project_impl_spec skenv_link (defs (Mod.get_sk md (Mod.data md)))); eauto. intro SPEC.
+    remember (SkEnv.project skenv_link (defs (Mod.get_sk md (Mod.data md)))) as skenv_proj eqn:T in *.
+    assert(WFSMALL: skenv_proj.(SkEnv.wf)).
+    { eapply SkEnv.project_spec_preserves_wf; eauto. }
+    clarify. des. inv SPEC.
+    exploit Genv.find_funct_inv; eauto. i; des. clarify. ss. des_ifs.
+    unfold Genv.find_funct_ptr in *. des_ifs.
+    inv WFSMALL. exploit DEFSYMB; eauto. intro SYMBSMALL; des.
+    assert((defs (Mod.get_sk md (Mod.data md))) id).
+    { apply NNPP. ii.
+      exploit SYMBDROP; eauto. i; des. clarify.
+    }
+    exploit SYMBKEEP; eauto. intro SYMBBIG; des.
+    rewrite SYMBSMALL in *. symmetry in SYMBBIG.
+    exploit DEFKEEP; eauto.
+    { eapply Genv.find_invert_symbol; eauto. }
+    intro DEFSMALL; des. rewrite Heq in *. symmetry in DEFSMALL.
+    clear - Heq0 DEFSMALL.
+    unfold System.skenv in *. ss.
+    exploit Genv_map_defs_spec; eauto. i; des. unfold System.gd_to_skd in MAP. des_ifs.
+    clear Heq0.
+    exploit Genv_map_defs_spec; eauto. i; des. des_ifs.
+  Qed.
+
+  (* Lemma link_sk_disjoint_aux *)
+  (*       (sks: list Sk.t) *)
+  (*       sk0 sk1 *)
+  (*       (IN0: In sk0 sks) *)
+  (*       (IN1: In sk1 sks) *)
+  (*       sk_link *)
+  (*       (LINKSK: link_list sks = Some sk_link) *)
+  (*       (NEQ: sk0 <> sk1) *)
+  (*   : *)
+  (*     sk0.(defs) /1\ sk1.(defs) <1= bot1 *)
+  (* . *)
+  (* Proof. *)
+  (*   admit "". *)
+  (* Qed. *)
+
+  (* Lemma link_sk_disjoint *)
+  (*       md0 md1 *)
+  (*       (IN0: In md0 p) *)
+  (*       (IN1: In md1 p) *)
+  (*       sk_link *)
+  (*       (LINKSK: link_sk p = Some sk_link) *)
+  (*       (NEQ: md0.(Mod.sk) <> md1.(Mod.sk)) *)
+  (*   : *)
+  (*     md0.(Mod.sk).(defs) /1\ md1.(Mod.sk).(defs) <1= bot1 *)
+  (* . *)
+  (* Proof. *)
+  (*   unfold link_sk in *. *)
+  (*   hexploit link_sk_disjoint_aux; eauto. *)
+  (*   { rewrite in_map_iff. esplits; eauto. } *)
+  (*   { rewrite in_map_iff. esplits; eauto. } *)
+  (* Qed. *)
+
+  Lemma link_sk_disjoint
+        md0 md1
+        (IN0: In md0 p)
+        (IN1: In md1 p)
+        sk_link
+        (LINKSK: link_sk p = Some sk_link)
+        (NEQ: md0 <> md1)
+    :
+      md0.(Mod.sk).(defs) /1\ md1.(Mod.sk).(defs) <1= bot1
+  .
+  Proof.
+    clear_tac. clear sem.
+    unfold link_sk in *.
+    unfold Mod.sk in *.
+    ginduction p; i; ss.
+    eapply link_list_cons_inv in LINKSK. des_safe.
+    hexploit (link_list_linkorder _ TL); eauto. intro TLORD; des_safe.
+    hexploit (link_linkorder _ _ _ HD); eauto. intro HDORD; des_safe.
+
+    destruct IN0; ss.
+    { clarify. des; ss.
+Local Transparent Linker_prog.
+      simpl in HD. simpl in TL.
+      ss.
+(* Local Opaque Linker_prog. *)
+(*       exploit link_prog_inv; eauto. *)
+(*       unfold Linker_prog in *. *)
+(*     } *)
+  Abort.
+
+  Theorem genv_disjoint
+    :
+      <<DISJ: sem.(globalenv).(Ge.disjoint)>>
+  .
+  Proof.
+    ss. des_ifs; cycle 1.
+    { econs; eauto. ii; ss. inv FIND0. ss. }
+    assert(WFBIG: t.(Sk.load_skenv).(SkEnv.wf)).
+    { eapply Sk.load_skenv_wf. }
+    econs; eauto.
+    ii; ss.
+    inv FIND0; inv FIND1.
+    unfold Sk.load_skenv in *. unfold load_genv in *. unfold load_modsems in *. ss.
+    abstr (Genv.globalenv t) skenv_link. rename t into sk_link.  rename Heq into SKLINK.
+    rewrite in_map_iff in *.
+    u in *.
+    destruct MODSEM.
+    { clarify. des; ss. exfalso. clarify. eapply system_disjoint; eauto. }
+    des; ss.
+    { clarify. ss. exfalso. eapply system_disjoint; eauto. }
+
+    rename x into md0. rename x0 into md1.
+    clarify.
+    destruct fptr; ss. des_ifs. unfold Genv.find_funct_ptr in *. des_ifs.
+    rename Heq0 into DEF0. rename Heq into DEF1.
+    rewrite <- Mod.get_modsem_projected_sk in *.
+    hexploit (SkEnv.project_impl_spec skenv_link (defs (Mod.get_sk md0 (Mod.data md0)))); eauto. intro SPEC0.
+    hexploit (SkEnv.project_impl_spec skenv_link (defs (Mod.get_sk md1 (Mod.data md1)))); eauto. intro SPEC1.
+    des.
+
+    assert(WFSMALL0: (SkEnv.project skenv_link (defs (Mod.get_sk md0 (Mod.data md0)))).(SkEnv.wf)).
+    { eapply SkEnv.project_spec_preserves_wf; try apply SPEC0; eauto. }
+    assert(WFSMALL1: (SkEnv.project skenv_link (defs (Mod.get_sk md1 (Mod.data md1)))).(SkEnv.wf)).
+    { eapply SkEnv.project_spec_preserves_wf; try apply SPEC1; eauto. }
+
+    bar.
+    inv WFSMALL0. exploit DEFSYMB; eauto. i; des.
+    inv WFSMALL1. exploit DEFSYMB0; eauto. i; des.
+    rename H into SYMB0. rename H1 into SYMB1. rename id0 into id1. rename id into id0.
+    move SYMB0 at top. move SYMB1 at top. clear_until_bar.
+
+    inv SPEC0.
+    assert(DEFS0: defs (Mod.get_sk md0 (Mod.data md0)) id0).
+    { apply NNPP. ii. exploit SYMBDROP; eauto. i; des. clarify. }
+    exploit SYMBKEEP; eauto. intro SYMBBIG0; des. rewrite SYMB0 in *. symmetry in SYMBBIG0.
+    exploit DEFKEEP; eauto.
+    { eapply Genv.find_invert_symbol; eauto. }
+    intro DEFBIG0; des. rewrite DEF0 in *. symmetry in DEFBIG0.
+    move SYMBBIG0 at top.
+    move DEFBIG0 at top.
+    move DEFS0 at top.
+    clear_until_bar.
+
+    inv SPEC1.
+    assert(DEFS1: defs (Mod.get_sk md1 (Mod.data md1)) id1).
+    { apply NNPP. ii. exploit SYMBDROP; eauto. i; des. clarify. }
+    exploit SYMBKEEP; eauto. intro SYMBBIG1; des. rewrite SYMB1 in *. symmetry in SYMBBIG1.
+    exploit DEFKEEP; eauto.
+    { eapply Genv.find_invert_symbol; eauto. }
+    intro DEFBIG1; des. rewrite DEF1 in *. symmetry in DEFBIG1.
+    move SYMBBIG1 at top.
+    move DEFBIG1 at top.
+    move DEFS1 at top.
+    clear_until_bar.
+
+    assert(id0 = id1).
+    { eapply Genv.genv_vars_inj.
+      { apply SYMBBIG0. }
+      { apply SYMBBIG1. }
+    } clarify.
+    rename id1 into id.
+
+    clear - DEF0 DEF1 DEFBIG0 DEFS0 DEFS1 SKLINK H0 MODSEM1.
+    destruct (classic (md0 = md1)); ss.
+    { clarify. }
+    admit "this should hold. state some lemma like: link_sk_disjoint".
+  Qed.
+
+  Lemma find_fptr_owner_determ
+        fptr ms0 ms1
+        (FIND0: Ge.find_fptr_owner sem.(globalenv) fptr ms0)
+        (FIND1: Ge.find_fptr_owner sem.(globalenv) fptr ms1)
+    :
+      ms0 = ms1
+  .
+  Proof.
+    inv FIND0; inv FIND1. ss. des_ifs.
+    unfold load_genv in *. ss.
+    admit "use Mod.get_modsem_projected_sk".
+  Qed.
+
+  Theorem initial_state_determ
+          st_init0 st_init1
+          (INIT0: sem.(Smallstep.initial_state) st_init0)
+          (INIT1: sem.(Smallstep.initial_state) st_init1)
+    :
+      st_init0 = st_init1
+  .
+  Proof.
+    ss.
+    inv INIT0; inv INIT1; ss.
+    clarify.
+    exploit find_fptr_owner_determ; ss; des_ifs.
+    { eapply MSFIND. }
+    { eapply MSFIND0. }
+    i; des. clarify.
+    determ_tac ModSem.initial_frame_dtm.
+  Qed.
+
+End INITDTM.
+
+
+
+
